\section{随机变量的分布函数}

% \subsection{二项分布}
% 
% 若 $X$ 的概率分布列为
% $$P\left( X=k\right) =\binom{n}{k}p^{k}\left( 1-p\right) ^{n-k}~ (k=0,1,\cdots ,n)$$
% 则称 $X$ 服从二项分布, 记为 $X\sim b(n,p)$, 其中 $0<p<1.$
% 
% \begin{example}
%     设随机变量 $X\sim b(n,p)$, 求 $E(X)$ 和 $D(X).$
% \end{example}
% \begin{solution}
%     由期望的定义, 
%     \begin{flalign*}
%         E\left( X\right) =\sum ^{n}_{k=0}k\binom{n}{k}p^{k}\left( 1-p\right) ^{n-k}=np\sum ^{n}_{k=1}\binom{n-1}{k-1}p^{k-1}\left( 1-p\right) ^{\left( n-1\right) -\left( k-1\right) }=np[p+(1-p)]^{n-1}=np,
%     \end{flalign*}
%     因为, $D(X)=E(X^2)-E^2(X)$, 下求 $E(X^2)$, 
%     \begin{flalign*}
%         E(X^2) & =\sum ^{n}_{k=0}k^{2}\binom{n}{k}p^{k}\left( 1-p\right) ^{n-k}=\sum ^{n}_{k=1}\left( k-1+1\right) k\binom{n}{k}p^{k}\left( 1-p\right) ^{n-k}                                                                \\
%                & =\sum ^{n}_{k=1}\left( k-1\right) k\binom{n}{k}p^{k}\left( 1-p\right) ^{n-k}+\sum ^{n}_{k=1}k\binom{n}{k}p^{k}\left( 1-p\right) ^{n-k}                                                                      \\
%                & =\sum ^{n}_{k=2}\left( k-1\right) k\binom{n}{k}p^{k}\left( 1-p\right) ^{n-k}+np\\
%                & =n\left( n-1\right) p^{2}\sum ^{n}_{k=2}\binom{n-2}{k-2}p^{k-2}\left( 1-p\right) ^{\left( n-2\right) -\left( k-2\right) }+np\\
%                & =n\left( n-1\right) p^{2}+np,
%     \end{flalign*}
%     故 $D(X)=n(n-1)p^2+np-(np)^2=np(1-p).$
% \end{solution}
% \begin{example}
%     设随机变量 $X\sim b(n,p)$, 已知 $E(X)=2.4,D(X)=1.44$, 求参数 $n$ 和 $p$.
% \end{example}
% \begin{solution}
%     因为 $E(X)=np,D(X)=np(1-p)$, 所以 $n=6,p=0.4.$
% \end{solution}
% 
% \subsection{0-1 分布}
% 
% \subsection{Poisson 分布}
% 
% \subsection{超几何分布}
% 
% \subsection{几何分布}
% 
% \subsection{负二项分布}